\documentclass{article}
\usepackage[norsk]{babel}
\selectlanguage{norsk}

\title{TDAT 2002 Matematikkprosjekt}
\author{Irrasjonelle Karer}
\date{Vår 2020}
\newpage

\begin{document}
        \maketitle
        \newpage
        \tableofcontents
        \newpage
        
        \section{Oppgave 1}
        \subsection{Teori}
        Taylors formel med restledd:
        \[R_5(x)= \frac{f^{(6)}(c)} {6!}(x-x_0)^6\]
        \[EIy''''=f(x)\]
        \[y''''(x) \approx \frac{y(x - 2h)-4y(x - h)+ 6y(x) - 4y(x + h) + y(x + 2h)}{h^4}\]
        \subsection{Oppgaveløsing}
    
    \subsubsection{Oppgave 5.1.21}
    \begin{enumerate}

        \item \[f(x + 2h) = f(x) + 2hf'(x) + 2h^2f''(x) + \frac{4}{3}h^3f'''(x)+ \frac{2}{3}n^4f''''(x) +O(n^6)\]
         \[f(x - 2h) = f(x) - 2hf'(x) + 2h^2f''(x) - \frac{4}{3}h^3f'''(x)+ \frac{2}{3}n^4f''''(x) +O(n^6)\]
         \[f(x + h) = f(x) + hf'(x) + \frac{1}{2}h^2f''(x) + \frac{1}{6}h^3f'''(x)+ \frac{1}{24}n^4f''''(x) +O(n^6)\]
         \[f(x - h) = f(x) - hf'(x) + \frac{1}{2}h^2f''(x) - \frac{1}{6}h^3f'''(x)+ \frac{1}{24}n^4f''''(x) +O(n^6)\]
        \item \[f(x + h) + f(x - h) + f(x + 2h) + f(x - 2h)\]
        \[= 4f(x) + 5h^2f'''(x) + \frac{17}{12}h^4f''''(x)\]
        \item \[f''(x)h = f(x - h) + f(x + h)\]
        \[=\]
        \[f(x) + hf'(x) + \frac{1}{2}h^2f''(x) + \frac{1}{6}h^3f'''(x)+ \frac{1}{24}n^4f''''(x)\]
        \[+\]
        \[f(x) - hf'(x) + \frac{1}{2}h^2f''(x) - \frac{1}{6}h^3f'''(x)+ \frac{1}{24}n^4f''''(x)\]
        \[= f(x) + hf'(x) + \frac{1}{2}h^2f''(x) + f(x) - hf'(x) + \frac{1}{2}h^2f''(x)\]
        \[= 2f(x) + h^2f''(x) + \frac{1}{2}h^4f''''(x)\]
        \item
        \[h^2f''(x) = 2f(x) - \frac{1}{12}h^4f''''(x) + f(x - h) + f(x + h)\]
        \[= 4f(x) + 5(-2f(x)-\frac{1}{12} h^4f''''(x)) + \frac{17}{12}h^4f''''(x)\]
        \[= 4f(x) - 10f(x) - \frac{5}{12}h^4f''''(x) + \frac{17}{12}h^4f''''(x)\]
        \[= -6f(x) + h^4f''''(x) + 5f(x - h) + 5f(x + h)\]
        \item \[f(x - 2h) + f(x - h) + f(x + h) + f(x + 2h) + 6f(x) - 5f(x - h) - 5f(x + h)\]
        \[f''''(x) = \frac{2(x-2h) - 4(x-h) + 6f(x) - 4(x+h) + f(x+h)} {h^4} = O(n^2)\]
    \end{enumerate}

    \subsubsection{Oppgave 5.1.22a}
    \[f(x) = f'(x) = 0\]
    then
    \[f''''(x+h) - \frac{16f(x+h) - 9f(x+2h) + \frac{8}{3}f(x+3h)-\frac{1}{4}f(x+4h)}{h^4}=O(h^2)\]
    \begin{enumerate}
    \item \[f(x-h)=f(x)-hf'(x) + \frac{1}{2}h^2f''(x)-\frac{1}{6}h^3f'''(x)+\frac{1}{24}h^4f''''(x)\]
    \[f''''(x-h) = f''''(x) + f^{(5)}(x) + \frac{1}{2}h^2f^{(6)}(x)+\frac{1}{6}h^3f^{(7)}(x)+\frac{1}{24}h^4f^{(8)}(x)\]
    \[f(x+h) = f(x)+hf(x) + \frac{1}{2}h^2f''(x)+\frac{1}{6}h^3f'''(x)+\frac{1}{24}h^4f''''(x)\]
    \[f(x+2h)=f(x)+2hf'(x)+2h^2f''(x)+\frac{4}{3}h^3f'''(x)+\frac{2}{3}h^4f''''(x)\]
    \[f(x+3h)=f(x) + 3hf'(x) + \frac{9}{2}h^2f''''(x)\frac{9}{2}h^3f'''(x)+\frac{27}{8}h^4f''''(x) + \frac{81h^5f^{(5)}(x)}{40}\]
    \[f(x+3h) = f(x)+4hf'(x)+8h^2f''(x) + \frac{32}{3}h^3f'''(x) + \frac{32}{3}h^4f''''(x) + \frac{128h^5f^{(5)}(x)}{15}\]
    
    \item  \[f''''(x-h) = f''''(x) + f^{(5)}(x) + O(h^2)\]
    \item \[f''''(x) + f^{(5)} + O(h^2)-\]
    \[16(\frac{1}{2}h^2f''(x))+\frac{1}{6}h^3f'''(x)+\frac{1}{24}h^4f''''(x)+\frac{1}{120}h^5f^{(5)}(x)+O(h^6))\]
    \[-9(2h^2f'(x)+\frac{4}{3}h^3f'''(x)+\frac{2}{3}h^4f''''(x)+\frac{4}{15}h^5f^{(5)}(x)+O(h^6))\]
    \[+\frac{8}{3}(\frac{9}{2}h^2f''(x)+\frac{9}{2}h^3f'''(x)+\frac{27}{8}h^4f''''(x) + \frac{81}{40}h^5f^{(5)}(x))+O(h^6)\]
    \[-\frac{1}{4}(8h^2f''(x)+\frac{32}{3}h^3+\frac{32}{3}h^4f''''(x)+\frac{128}{15}h^5f^{(5)}(x)+O(h^6))\]
    \[= \]
    
    \end{enumerate}

    \begin{flushleft}
        
    $\frac{f''''(x) + f^{(5)}(x) + O(h^2) - (8-18+12-2)h^2f''(x)+(\frac{8}{3}+12-12-\frac{8}{3})f'''(x) + (\frac{2}{3}-6+9-\frac{8}{3}) f''''(x)+(\frac{2}{15}-\frac{12}{5}+\frac{21}{5} - \frac{32}{15})f^{(5)}(x)}{h^4}$
    $= f''''(x)+f^{(5)}(x)+O(h^2) - f''''(x) - f^{(5)}(x) = O(h^2)$
    \end{flushleft}

    \section{Oppgave 2}

    \section{Oppgave 3}

    \section{Oppgave 4}
    \subsection{Teori}

    \subsection{Oppgaveløsing}

    \subsubsection{a}
    \[f(x) = f\]
    \[EIy''''=f(x)\]
    \[y(x)=(\frac{f}{24EI})x^2(x^2-4Lx+6L^2)\]
    \[y''''(x) = \frac{f}{24EI}24\]
    \[EIy''''(x) = f\]
    \subsubsection{b}
    \[\frac{y^{(6)}(l)}{6!}h^6\]
    Videre derivering av $y$ vil bli $0$. 
    $\frac{Ay}{h^4}$ er det vi gjorde i \emph{Oppgave 1, seksjon 1.2.2}.  
    Den vil blir eksakt, da $O(h^6) = 0$
    \section{Oppgave 5}

    \section{Oppgave 6}

    \section{Oppgave 7}

    
   

    

        

        

\end{document}