\documentclass[11pt]{article}
\title{Oppgave 1}
\begin{document}

        \section{Teori}
        Taylors formel med restledd:
        \[R_5(x)= \frac{f^{(6)}(c)} {6!}(x-x_0)^6\]
        \[EIy''''=f(x)\]
        \[y''''(x) \approx \frac{y(x - 2h)-4y(x - h)+ 6y(x) - 4y(x + h) + y(x + 2h)}{h^4}\]
        \section{Oppgavel√∏sing}
    
    \textbf{Oppgave 5.1.21}
    \begin{enumerate}

        \item \[f(x + 2h) = f(x) + 2hf'(x) + 2h^2f''(x) + \frac{4}{3}h^3f'''(x)+ \frac{2}{3}n^4f''''(x) +O(n^6)\]
         \[f(x - 2h) = f(x) - 2hf'(x) + 2h^2f''(x) - \frac{4}{3}h^3f'''(x)+ \frac{2}{3}n^4f''''(x) +O(n^6)\]
         \[f(x + h) = f(x) + hf'(x) + \frac{1}{2}h^2f''(x) + \frac{1}{6}h^3f'''(x)+ \frac{1}{24}n^4f''''(x) +O(n^6)\]
         \[f(x - h) = f(x) - hf'(x) + \frac{1}{2}h^2f''(x) - \frac{1}{6}h^3f'''(x)+ \frac{1}{24}n^4f''''(x) +O(n^6)\]
        \item \[f(x + h) + f(x - h) + f(x + 2h) + f(x - 2h)\]
        \[= 4f(x) + 5h^2f'''(x) + \frac{17}{12}h^4f''''(x)\]
        \item \[f''(x)h = f(x - h) + f(x + h)\]
        \[=\]
        \[f(x) + hf'(x) + \frac{1}{2}h^2f''(x) + \frac{1}{6}h^3f'''(x)+ \frac{1}{24}n^4f''''(x)\]
        \[+\]
        \[f(x) - hf'(x) + \frac{1}{2}h^2f''(x) - \frac{1}{6}h^3f'''(x)+ \frac{1}{24}n^4f''''(x)\]
        \[= f(x) + hf'(x) + \frac{1}{2}h^2f''(x) + f(x) - hf'(x) + \frac{1}{2}h^2f''(x)\]
        \[= 2f(x) + h^2f''(x) + \frac{1}{2}h^4f''''(x)\]
        \item
        \[h^2f''(x) = 2f(x) - \frac{1}{12}h^4f''''(x) + f(x - h) + f(x + h)\]
        \[= 4f(x) + 5(-2f(x)-\frac{1}{12} h^4f''''(x)) + \frac{17}{12}h^4f''''(x)\]
        \[= 4f(x) - 10f(x) - \frac{5}{12}h^4f''''(x) + \frac{17}{12}h^4f''''(x)\]
        \[= -6f(x) + h^4f''''(x) + 5f(x - h) + 5f(x + h)\]
        \item \[f(x - 2h) + f(x - h) + f(x + h) + f(x + 2h) + 6f(x) - 5f(x - h) - 5f(x + h)\]
        \[f''''(x) = \frac{2(x-2h) - 4(x-h) + 6f(x) - 4(x+h) + f(x+h)} {h^4} = O(n^2)\]
        
    \end{enumerate}

    \textbf{Oppgave 5.1.22a}

    \[f(x) = f'(x) = 0\]
    then
    \[f''''(x+h) - \frac{16f(x+h) - 9f(x+2h) + \frac{8}{3}f(x+3h)-\frac{1}{4}f(x+4h)}{h^4}=O(h^2)\]

    \begin{enumerate}
        \item 
    \end{enumerate}

        

        

\end{document}